WIP

src/refinement/SimCertify.v
@@ -10,6 +10,7 @@ Require Import ZArith.
 Require Import FMapPositive.
 Require Import FSetPositive.
 Require Import EquivDec.
+Require Import HahnSets.
 Require Import sflib.
 
 Require Import Basic.
@@ -28,48 +29,52 @@ Inductive sim_time (ts:Time.t) (v1 v2:Time.t): Prop :=
 .
 Hint Constructors sim_time.
 
-Inductive sim_view (ts:Time.t) (v1 v2:View.t (A:=Taint.t)): Prop :=
+Inductive sim_view (ts:Time.t) (ex:Taint.t) (v1 v2:View.t (A:=Taint.t)): Prop :=
 | sim_view_intro
-    (TS: v2.(View.ts) <= ts -> v1 = v2)
+    (TS: v2.(View.ts) <= ts ->
+         v1 = v2 /\
+         v2.(View.annot) ∩₁ ex = bot)
 .
 Hint Constructors sim_view.
 
-Inductive sim_val (ts:Time.t) (v1 v2:ValA.t (A:=View.t (A:=Taint.t))): Prop :=
+Inductive sim_val (ts:Time.t) (ex:Taint.t) (v1 v2:ValA.t (A:=View.t (A:=Taint.t))): Prop :=
 | sim_val_intro
-    (TS: v2.(ValA.annot).(View.ts) <= ts -> v1 = v2)
+    (TS: v2.(ValA.annot).(View.ts) <= ts ->
+         v1 = v2 /\
+         v2.(ValA.annot).(View.annot) ∩₁ ex = bot)
 .
 Hint Constructors sim_val.
 
-Inductive sim_rmap (ts:Time.t) (rmap1 rmap2:RMap.t (A:=View.t (A:=Taint.t))): Prop :=
+Inductive sim_rmap (ts:Time.t) (ex:Taint.t) (rmap1 rmap2:RMap.t (A:=View.t (A:=Taint.t))): Prop :=
 | sim_rmap_intro
     (RMAP: IdMap.Forall2
-             (fun _ => (sim_val ts))
+             (fun _ => (sim_val ts ex))
              rmap1 rmap2)
 .
 Hint Constructors sim_rmap.
 
-Inductive sim_state (ts:Time.t) (st1 st2:State.t (A:=View.t (A:=Taint.t))): Prop :=
+Inductive sim_state (ts:Time.t) (ex:Taint.t) (st1 st2:State.t (A:=View.t (A:=Taint.t))): Prop :=
 | sim_state_intro
     (STMTS: st1.(State.stmts) = st2.(State.stmts))
-    (RMAP: sim_rmap ts st1.(State.rmap) st2.(State.rmap))
+    (RMAP: sim_rmap ts ex st1.(State.rmap) st2.(State.rmap))
 .
 Hint Constructors sim_state.
 
-Inductive sim_lc (ts:Time.t) (lc1 lc2:Local.t (A:=Taint.t)): Prop :=
+Inductive sim_lc (ts:Time.t) (ex:Taint.t) (lc1 lc2:Local.t (A:=Taint.t)): Prop :=
 | sim_lc_intro
     (COH: forall loc, sim_time ts (lc1.(Local.coh) loc) (lc2.(Local.coh) loc))
-    (VRP: sim_view ts lc1.(Local.vrp) lc2.(Local.vrp))
-    (VWP: sim_view ts lc1.(Local.vwp) lc2.(Local.vwp))
-    (VRM: sim_view ts lc1.(Local.vrm) lc2.(Local.vrm))
-    (VWM: sim_view ts lc1.(Local.vwm) lc2.(Local.vwm))
-    (VCAP: sim_view ts lc1.(Local.vcap) lc2.(Local.vcap))
-    (VREL: sim_view ts lc1.(Local.vrel) lc2.(Local.vrel))
+    (VRP: sim_view ts ex lc1.(Local.vrp) lc2.(Local.vrp))
+    (VWP: sim_view ts ex lc1.(Local.vwp) lc2.(Local.vwp))
+    (VRM: sim_view ts ex lc1.(Local.vrm) lc2.(Local.vrm))
+    (VWM: sim_view ts ex lc1.(Local.vwm) lc2.(Local.vwm))
+    (VCAP: sim_view ts ex lc1.(Local.vcap) lc2.(Local.vcap))
+    (VREL: sim_view ts ex lc1.(Local.vrel) lc2.(Local.vrel))
     (FWDBANK: forall loc,
         opt_rel
           (fun fwd1 fwd2 =>
              fwd2.(FwdItem.ts) <= ts ->
              (fwd1.(FwdItem.ts) = fwd2.(FwdItem.ts) /\
-              sim_view ts fwd1.(FwdItem.view) fwd2.(FwdItem.view) /\
+              sim_view ts ex fwd1.(FwdItem.view) fwd2.(FwdItem.view) /\
               fwd1.(FwdItem.ex) = fwd2.(FwdItem.ex)))
           (lc1.(Local.fwdbank) loc) (lc2.(Local.fwdbank) loc))
     (EXBANK: opt_rel
@@ -80,25 +85,160 @@ Inductive sim_lc (ts:Time.t) (lc1 lc2:Local.t (A:=Taint.t)): Prop :=
 .
 Hint Constructors sim_lc.
 
-Inductive sim_mem (ts:Time.t) (mem1 mem2:Memory.t): Prop :=
+Inductive sim_mem (tid:Id.t) (ts:Time.t) (ex:Taint.t) (mem1 mem2:Memory.t): Prop :=
 | sim_mem_intro
-    (LEN: ts <= length mem1)
-    (LEN: ts <= length mem2)
-    (MEM: firstn ts mem1 = firstn ts mem2)
+    mem_prefix mem1' mem2' msg
+    (LEN: ts = length mem_prefix)
+    (MEM: mem1 = mem_prefix ++ mem1')
+    (MEM: mem2 = mem_prefix ++ msg :: mem2')
+    (MSG: msg.(Msg.tid) <> tid)
+    (EX: ex = (fun taint => exists id, taint = Taint.R id 0))
 .
 Hint Constructors sim_mem.
 
-Inductive sim_eu (ts:Time.t) (eu1 eu2:ExecUnit.t (A:=Taint.t)): Prop :=
+Inductive sim_eu (tid:Id.t) (ts:Time.t) (ex:Taint.t) (eu1 eu2:ExecUnit.t (A:=Taint.t)): Prop :=
 | sim_eu_intro
-    (STATE: sim_state ts eu1.(ExecUnit.state) eu2.(ExecUnit.state))
-    (LOCAL: sim_lc ts eu1.(ExecUnit.local) eu2.(ExecUnit.local))
-    (MEM: sim_mem ts eu1.(ExecUnit.mem) eu2.(ExecUnit.mem))
+    (STATE: sim_state ts ex eu1.(ExecUnit.state) eu2.(ExecUnit.state))
+    (LOCAL: sim_lc ts ex eu1.(ExecUnit.local) eu2.(ExecUnit.local))
+    (MEM: sim_mem tid ts ex eu1.(ExecUnit.mem) eu2.(ExecUnit.mem))
 .
 Hint Constructors sim_eu.
 
-Inductive sim_aeu (ts:Time.t) (aeu1 aeu2:AExecUnit.t): Prop :=
+Inductive sim_aeu (tid:Id.t) (ts:Time.t) (ex:Taint.t) (aeu1 aeu2:AExecUnit.t): Prop :=
 | sim_aeu_intro
-    (EU: sim_eu ts aeu1.(AExecUnit.eu) aeu2.(AExecUnit.eu))
+    (EU: sim_eu tid ts ex aeu1.(AExecUnit.eu) aeu2.(AExecUnit.eu))
     (AUX: aeu1.(AExecUnit.aux) = aeu2.(AExecUnit.aux))
+    (AUX_EX: aeu2.(AExecUnit.aux).(AExecUnit.taint) ∩₁ ex ⊆₁ bot)
 .
 Hint Constructors sim_aeu.
+
+Lemma sim_aeu_step
+      tid ts ex aeu1 aeu2 aeu2'
+      (SIM: sim_aeu tid ts ex aeu1 aeu2)
+      (STEP: AExecUnit.step tid aeu2 aeu2'):
+  exists aeu1',
+    <<STEP: AExecUnit.step tid aeu1 aeu1'>> /\
+    <<SIM: sim_aeu tid ts ex aeu1' aeu2'>>.
+Proof.
+  destruct aeu1 as [[[stmts1 rmap1] lc1 mem1] aux1].
+  destruct aeu2 as [[[stmts2 rmap2] lc2 mem2] aux2].
+  destruct aeu2' as [[[stmts2' rmap2'] lc2' mem2'] aux2'].
+  inv STEP.
+  - (* state_step *)
+    inv STEP0. ss. subst.
+    inv SIM. ss. subst.
+    inv EU. ss.
+    inv STATE0. ss. subst.
+    inv STATE; inv LOCAL; inv H0.
+    + (* skip *)
+      inv LC.
+      eexists (AExecUnit.mk (ExecUnit.mk _ _ _) _). esplits.
+      * left. econs; ss.
+        { instantiate (2 := Event.internal bot). s. econs 1. }
+        econs; eauto. econs; eauto.
+      * econs; ss. econs; ss. econs; try by apply LOCAL0.
+        s. rewrite ? bot_join; try by apply View.order. apply LOCAL0.
+    + (* assign *)
+      inv LC.
+      eexists (AExecUnit.mk (ExecUnit.mk _ _ _) _). esplits.
+      * left. econs; ss.
+        { instantiate (2 := Event.internal bot). s. econs 2. eauto. }
+        econs; eauto. econs; eauto.
+      * econs; ss. econs; ss.
+        { econs; ss. admit. (* sim_rmap add *) }
+        { econs; try by apply LOCAL0.
+          s. rewrite ? bot_join; try by apply View.order. apply LOCAL0.
+        }
+    + (* read *)
+      admit.
+    + (* fulfill *)
+      admit.
+    + (* write_failure *)
+      inv STEP.
+      eexists (AExecUnit.mk (ExecUnit.mk _ _ _) _). esplits.
+      * left. econs; ss.
+        { instantiate (2 := Event.write _ _ _ _ _). s. econs 4; eauto. }
+        econs 4; eauto. econs; eauto.
+      * econs; ss; cycle 1.
+        { admit. (* join bot *) }
+        econs; ss.
+        { econs; ss. admit. (* sim_rmap add *) }
+        { econs; try by apply LOCAL0. ss. }
+    + (* isb *)
+      admit.
+    + (* dmbst *)
+      admit.
+    + (* dmbld *)
+      admit.
+    + (* dmbsy *)
+      admit.
+    + (* if *)
+      inv LC.
+      eexists (AExecUnit.mk (ExecUnit.mk _ _ _) _). esplits.
+      * left. econs; ss.
+        { instantiate (2 := Event.internal _). s. econs 6; eauto. }
+        econs; eauto. econs; eauto.
+      * econs; ss. econs; ss.
+        { econs; ss. admit. (* sim_rmap add *) }
+        { econs; try by apply LOCAL0. s.
+          admit. (* sim_view join *)
+        }
+    + (* dowhile *)
+      inv LC.
+      eexists (AExecUnit.mk (ExecUnit.mk _ _ _) _). esplits.
+      * left. econs; ss.
+        { instantiate (2 := Event.internal bot). s. econs 7. ss. }
+        econs; eauto. econs; eauto.
+      * econs; ss. econs; ss. econs; try by apply LOCAL0.
+        s. rewrite ? bot_join; try by apply View.order. apply LOCAL0.
+  - (* write_step *)
+    admit.
+Admitted.
+
+Lemma sim_aeu_rtc_step
+      tid ts ex aeu1 aeu2 aeu2'
+      (SIM: sim_aeu tid ts ex aeu1 aeu2)
+      (STEP: rtc (AExecUnit.step tid) aeu2 aeu2'):
+  exists aeu1',
+    <<STEP: rtc (AExecUnit.step tid) aeu1 aeu1'>> /\
+    <<SIM: sim_aeu tid ts ex aeu1' aeu2'>>.
+Proof.
+  revert aeu1 SIM. induction STEP.
+  { i. esplits; eauto. }
+  i. exploit sim_aeu_step; eauto. i. des.
+  exploit IHSTEP; eauto. i. des.
+  esplits; [|by eauto]. econs; eauto.
+Qed.
+
+Lemma certify_lift_diff
+      tid eu1 eu2 locks msg
+      (CERTIFY: certify tid eu2 locks)
+      (ST: eu2.(ExecUnit.state) = eu1.(ExecUnit.state))
+      (LC: eu2.(ExecUnit.local) = eu1.(ExecUnit.local))
+      (MEM: eu2.(ExecUnit.mem) = eu1.(ExecUnit.mem) ++ [msg])
+      (MSG: msg.(Msg.tid) <> tid):
+  <<CERTIFY: certify tid eu1 locks>> /\
+  <<NOLOCK: forall lock (LOCK: locks lock), ~ (lock.(Lock.loc) = msg.(Msg.loc) /\ lock.(Lock.from) = 0)>>.
+Proof.
+  destruct eu1 as [st1 lc1 mem1].
+  destruct eu2 as [st2 lc2 mem2].
+  ss. subst. inv CERTIFY.
+  exploit sim_aeu_rtc_step; eauto.
+  { instantiate (1 := AExecUnit.init (ExecUnit.mk st1 lc1 mem1)). econs; ss.
+    - econs; ss; cycle 2.
+      + econs; ss. rewrite List.app_nil_r. ss.
+      + econs; ss. econs. ii.
+        unfold AExecUnit.init_rmap. rewrite IdMap.map_spec.
+        destruct (IdMap.find id (State.rmap st1)); ss. econs. econs; ss.
+        splits; ss.
+        admit. (* but cap X = bot *)
+      + admit. (* sim_lc *)
+    - admit. (* but cap X = bot *)
+  }
+  i. des. esplits.
+  - econs; eauto.
+    + inv SIM. inv EU. inv LOCAL. etrans; eauto.
+    + inv SIM. congr.
+  - ii. des. destruct lock as [loc from to guarantee]. ss. subst.
+    inv LOCK. ss. inv SIM. eapply AUX_EX. econs; cycle 1; eauto.
+Qed.
